\section{Question 17}
\horz

Let $\lambda = \{\lambda_j\}_{j\in \mathbb N}$ be sequence in $\ell^{\infty}(\mathbb N).$ Consider the unilateral weighted shift operator $W_{\lambda}$ on $\ell^2(\mathbb N)$ defined by 
\begin{align*}
W_{\lambda} (e_j)= \lambda_j e_{j+1},~~j\in \mathbb N,
\end{align*}
and extend linearly, that is, 
\begin{align*}
W_{\lambda} (c_1,c_2,c_3,\ldots)= (0,c_1\lambda_1,c_2\lambda_2,c_3\lambda_3,\ldots)
\end{align*}
Prove that the adjoint of $W_{\lambda}$ on $\ell^2(\mathbb N)$ is given by
\begin{align*}
W_{\lambda}^*(c_1,c_2,c_3,\ldots) = (c_2\overline{\lambda_1},c_3\overline{\lambda_2},c_4\overline{\lambda_3},\ldots).
\end{align*}
Moreover show that $\|W_{\lambda}\|= \|\lambda\|_{\infty} = \sup \{ |\lambda_j| : j\in \mathbb N\}.$

\horz
\begin{proof}
    Let $\left( c_{1}, c_{2}, \ldots \right)$ and $\left( d_{1}, d_{2}, \ldots \right) \in \ell ^{2} \left( \N \right)$. Then consider the following:

    \begin{align*}
	\ip{\left( c_{1}, c_{2}, \ldots \right), W_{\lambda}^{*} \left( d_{1}, d_{2}, \ldots \right)} &= \ip{W_{\lambda} \left( c_{1}, c_{2}, \ldots \right), (d_{1}, d_{2}, \ldots )} \\
    &= \ip{ \left( 0, c_{1}\lambda_{1}, c_{2} \lambda_{2}, \ldots ), \left( d_{1}, d_{2}, d_{3}, \ldots \right) \right) } \\
    &= c_{1} \lambda_{1} \bar{d_{2}} + c_{2} \lambda_{2} \bar{d_{3}} + \ldots \\
    &= \ip{(c_{1}, c_{2}, \ldots ), \left( \bar{\lambda_{1}} d_{2}, \bar{\lambda_{2}} d_{3} , \ldots \right)}.
    \end{align*}
    Since $\left( c_{i} \right)$ and $\left( d_{i} \right)$ were arbitrary, we have that 
    \begin{equation*}
	W_{\lambda} ^{*} \left( d_{1}, d_{2}, \ldots \right) = \left( \bar{\lambda_{1}} d_{2}, \bar{\lambda_{2}}d_{3}, \ldots \right) 
    \end{equation*}
    for each $\left( d_{1}, d_{2}, \ldots \right) \in \ell ^{2} \left( \N \right)$.

    Now, observe that $W_{\lambda} \left( e_{i} \right) = \lambda_{i}$ for each $i\in \N$. Thus, we have that
    \begin{equation*}
	\norm{\lambda}_{\infty} = \sup_{j \in \N} {\abs{\lambda_{j}}} \le \norm{W_{\lambda}}.
    \end{equation*}
    To show the reverse inequality, let $\left( c_{1}, c_{2}, \ldots \right) \in \ell ^{2} \left( \N \right)$. Then we have that 
    \begin{align*}
	\norm{W_{\lambda} \left( c_{1}, c_{2}, \ldots \right)}_{2} ^{2} &= \sum_{i=1}^{\infty} \abs{\lambda _{i} c_{i}}^{2} \\
	&\le \sup_{i\in \N} \abs{\lambda_{i}}^{2} \sum_{i=1}^{\infty} \abs{c_{i}}^{2} \\
	&= \norm{\lambda}_{\infty}^{2} \norm{\left( c_{1}, c_{2}, \ldots \right)}_{2}
    \end{align*}
    This implies that $\norm{W_{\lambda}} \le \norm{\lambda}_{\infty}$. This completes the proof.
\end{proof}
