\section{Question 4}
\horz

Let $H$ be a Hilbert space and $P_1, P_2\in \mathcal B(H),$ are two orthogonal projections,that is, $P_j^2=P_j$ and $P_j^*=P_j$ for each $j=1,2$. Show that $P_1P_2$ is an orthogonal projection if and only if $P_1P_2= P_2P_1.$ In this case $\operatorname{ran} (P_1P_2)= \operatorname{ran} (P_1) \cap \operatorname {ran}(P_2).$

\horz

\begin{proof}
    Let $P_{1}, P_{2} \in \calB \left( H \right)$ be two orthogonal projections.
    We show that $P_{1} P_{2}$ is an orthogonal projection iff $P_{1} P_{2} = P_{2} P_{1}$. 

    $\left( \Longrightarrow \right)$ Suppose that $P_{1} P_{2}$ is an orthogonal projection. We wish to show that $P_{1} P_{2} = P_{2} P_{1}$. To do so, consider the following:
    \begin{align*}
	P_{1} P_{2} &= \left( P_{1} P_{2} \right) ^{*} & P_{1} P_{2} \text{ being orthogonal projection} \\
	&= P_{2}^{*} P_{1} ^{*} & \text{property of the adjoint}\\
	&= P_{2} P_{1} & P_{1}, P_{2}. \text{ being orthogonal projection}
    \end{align*}
    $\left( \Longleftarrow \right)$ Suppose that $P_{1} P_{2} = P_{2} P_{1}$. We wish to show that $P_{1}P_{2}$ is an orthogonal projection. 
    \begin{description}
	\item[$P_{1}P_{2}$ is self adjoint:] Consider the following:
	    \begin{align*}
		(P_{1} P_{2})^{*} &= P_{2}^{*} P_{1} ^{*} \\
		&= P_{2} P_{1} \\
		&= P_{1} P_{2}. & \text{ by assumption }
	    \end{align*}

	\item[$P_{1} P_{2}$ is idempotent:] Consider the following:
	    \begin{align*}
		(P_{1} P_{2})^{2} &= P_{1} P_{2} P_{1} P_{2} \\
		&= P_{1} P_{1} P_{2} P_{2} & \text{since } P_{1} P_{2} = P_{2} P_{1} \\
		&= P_{1}^{2} P_{2}^{2} \\
		&= P_{1} P_{2} & \text{since } P_{1}, P_{2} \text{ are orthogonal projection}
	    \end{align*}
    \end{description}
    This shows that the both directions of the iff.
    Let us assume that $P_{1}P_{2}=P_{2}P_{1}$. Now, we proceed to show that $\im \left( P_{1} P_{2} \right) = \im P_{1} \cap \im P_{2}$. 
    \begin{description}
	\item[$(\subset)$ :] Let $y \in \im P_{1}P_{2}$. Then we have that $y=P_{1}P_{2} x$ for some $x\in H$. Since $P_{2}x \in H$, we have that $y=P_{1}x$. Also, note that $y=P_{2}P_{1}x$ since $P_{1}$ and $P_2$ commute. Hence, we have that $y\in \im P_{2}$. This shows that $\im P_{1}P_{2} \subset \im P_{1} \cap \im P_{2}$.
	\item[$(\supset)$ :] Let $y\in \im P_{1} \cap \im P_{2}$. Then we have $y=P_{1}x_{1}=P_{2}x_{2}$ for some $x_{1} \in H$ and some $x_{2} \in H$. It follows that
	    \begin{align*}
		P_{1}y &=P_{1}^{2} x_{1} \leadsto P_{1}y = P_{1}x_{1} \leadsto y= P_{1}y
	    \end{align*}
	    and
\begin{align*}
    P_{2}y &=P_{2}^{2} x_{2} \leadsto P_{2}y = P_{2}x_{2} \leadsto y= P_{2}y.
	    \end{align*}
	    The above two equalities show that $y\in \im P_{1} \cap \im P_{2}$.
    \end{description}
\end{proof}

